finish Cv1_Axiom theorem, make type_CvTheory build
I think this completes all the required theorems (case_def and case_cong
follow automatically from Axiom).
Now need to figure out how to emulate Hol_datatype's work to put stuff
into the TypeBase and make it persistent.

examples/miniML/compiler/type_CvScript.sml
@@ -1,4 +1,4 @@
-open HolKernel bossLib fmaptreeTheory finite_mapTheory pred_setTheory lcsymtacs
+open HolKernel boolLib bossLib fmaptreeTheory finite_mapTheory pred_setTheory lcsymtacs
 val _ = new_theory"type_Cv"
 
 val _ = Parse.overload_on("num_to_s0",``GENLIST (K (CHR 0))``)
@@ -10,7 +10,7 @@ num +
 string list # α +
 string list # (string list # α) list # string``
 val Cv0 = ``:(^b,^a) fmaptree``
-val _ = type_abbrev("Cv0",Cv0)
+val _ = Parse.type_abbrev("Cv0",Cv0)
 val Cvwf_def = new_specification("Cvwf_def",["Cvwf"],
 fmtree_Axiom
 |> Q.ISPEC
@@ -235,6 +235,15 @@ unabbrev_all_tac >>
 rw[FUN_FMAP_DEF,listTheory.EL_MAP] )
 val _ = export_rewrites["Cvwf_constructors"]
 
+val fromCv1_thm = store_thm(
+"fromCv1_thm",``
+(fromCv1 (CLitv l) = ^(rand(rhs(concl(SPEC_ALL CLitv_def))))) ∧
+(fromCv1 (CConv n vs) = ^(rand(rhs(concl(SPEC_ALL CConv_def))))) ∧
+(fromCv1 (CClosure env xs b) = ^(rand(rhs(concl(SPEC_ALL CClosure_def))))) ∧
+(fromCv1 (CRecClos env ns defs d) = ^(rand(rhs(concl(SPEC_ALL CRecClos_def)))))``,
+rw[CLitv_def, CConv_def, CClosure_def, CRecClos_def,
+   GSYM (CONJUNCT2 Cv1_bij_thm)])
+
 val Cv1_11 = store_thm(
 "Cv1_11",``
 (∀l1 l2.
@@ -319,6 +328,18 @@ val Cv1_nchotomy = store_thm(
   (∃env ns defs n. Cv1 = CRecClos env ns defs n)``,
 ho_match_mp_tac Cv1_nice_ind >> rw[])
 
+val toCv1_o_fromCv1 = store_thm(
+"toCv1_o_fromCv1",
+``toCv1 o fromCv1 = I``,
+rw[FUN_EQ_THM,Cv1_bij_thm])
+val _ = export_rewrites["toCv1_o_fromCv1"]
+
+val I_o_f = store_thm(
+"I_o_f",
+``I o_f fm = fm``,
+rw[GSYM fmap_EQ_THM])
+val _ = export_rewrites["I_o_f"]
+
 val Cv1_Axiom = store_thm(
 "Cv1_Axiom",
 ``∀f0 f1 f2 f3 f4 f5 f6 f7.
@@ -331,18 +352,64 @@ val Cv1_Axiom = store_thm(
 (∀v vs. fn1 (v::vs) = f5 v vs (fn0 v) (fn1 vs)) ∧
 (∀env. fn2 env = f6 env (f7 o_f env))``,
 rw[] >>
+qho_match_abbrev_tac `∃fn0. P fn0` >>
+qsuff_tac `∃fn0. P (fn0 o fromCv1)` >- PROVE_TAC[] >>
+qunabbrev_tac `P` >>
+fs[fromCv1_thm] >>
+CONV_TAC (RESORT_EXISTS_CONV (fn [x,y,z] => [z,x,y])) >>
+qexists_tac `λenv. f6 env (f7 o_f env)` >> rw[] >>
+qho_match_abbrev_tac `∃fn0 fn1. P fn0 fn1` >>
+qsuff_tac `∃fn1 fn0. P fn0 (λvs. fn1 vs (MAP (fn0 o fromCv1) vs))` >- PROVE_TAC[] >>
+Q.ISPECL_THEN [`λr0:α list. f4`,`λv vs r r0. f5 v vs (HD r0) (r (TL r0))`] strip_assume_tac listTheory.list_Axiom >>
+qexists_tac `fn` >>
+qunabbrev_tac `P` >>
+fs[] >>
+qexists_tac `fmtreerec
+  (λi res fm.
+    case i of
+    | (INL l) => f0 l
+    | (INR (INL m)) =>
+      let vs =
+        (MAP toCv1 (GENLIST (FAPPLY fm o num_to_s0) (CARD (FDOM fm))))
+      in f1 m vs (fn vs (GENLIST (FAPPLY res o num_to_s0) (CARD (FDOM res))))
+    | (INR (INR (INL (xs,b)))) =>
+      let env = toCv1 o_f fm in
+      f2 env xs b (f6 env (f7 o_f env))
+    | (INR (INR (INR (ns,defs,d)))) =>
+      let env = toCv1 o_f fm in
+      f3 env ns defs d (f6 env (f7 o_f env)))` >>
+rw[fmtreerec_thm,LET_THM] >>
+rw[listTheory.MAP_GENLIST] >>
+qmatch_abbrev_tac `f1 m vs' (fn vs' gl) = f1 m vs (fn vs ml)` >>
+`vs' = vs` by (
+  unabbrev_all_tac >>
+  rw[listTheory.LIST_EQ_REWRITE,CARD_INJ_IMAGE,num_to_s0_inj] >>
+  rw[Cv1_bij_thm] >>
+  qmatch_abbrev_tac `FUN_FMAP w y ' z = Z` >>
+  `z ∈ y` by (
+    unabbrev_all_tac >> rw[] >> PROVE_TAC[] ) >>
+  unabbrev_all_tac >>
+  rw[FUN_FMAP_DEF] ) >>
+rw[] >>
+AP_TERM_TAC >>
+AP_TERM_TAC >>
+unabbrev_all_tac >>
+fs[CARD_INJ_IMAGE,num_to_s0_inj] >>
+rw[listTheory.LIST_EQ_REWRITE,listTheory.EL_MAP] >>
+AP_TERM_TAC >>
+rw[Cv1_bij_thm] >>
+AP_TERM_TAC >>
+qmatch_abbrev_tac `FUN_FMAP w y ' z = Z` >>
+`z ∈ y` by (
+  unabbrev_all_tac >> rw[] >> PROVE_TAC[] ) >>
+unabbrev_all_tac >>
+rw[FUN_FMAP_DEF] >>
+rw[Cv1_bij_thm])
 
+val [Cv1_case_def] = Prim_rec.define_case_constant Cv1_Axiom
+val Cv1_case_cong = save_thm(
+"Cv1_case_cong",
+Prim_rec.case_cong_thm Cv1_nchotomy Cv1_case_def)
+val _ = DefnBase.export_cong"Cv1_case_cong"
 
-val Cv1_case_def = Prim_rec.define_case_constant Cv1_Axiom
-val Cv1_case_cong = Prim_rec.case_cong_thm Cv1_nchotomy Cv1_case_def
-
-TypeBasePure.gen_datatype_info
-{ax=Cv1_Axiom, ind=Cv1_induction0, case_defs=Prim_rec.define_case_constant Cv1_Axiom}
-
-(*
-type Cv =
-  | CLitv of lit
-  | CConv of num * Cv list
-  | CClosure of (string,Cv) alist * string list * Cexp
-  | CRecClos of (string,Cv) alist * string list * (string list * Cexp) list * string
-*)
+val _ = export_theory()
